Experiment with the 'shifting' relation. Represent in a way so that it is a total rather than partial bijection

Common/Renaming.v
@@ -10,60 +10,186 @@ Require Import CompCert.Events.
 Require Import Lib.Extra.
 From mathcomp Require Import ssreflect ssrnat eqtype path ssrfun seq fingraph fintype.
 
-Section Renaming.
-
 Definition addr_t : Type := (Component.id * Block.id).
-  (* It seems only Block.id will need to be renamed.
+(* It seems only Block.id will need to be renamed.
      However, to compute a renaming, we have to know which "component memory" we are
      considering. To know the component memory, we need the Component.id.
+*)
+
+Section ShiftingAsPartialBijection.
+  (* The following is a definition of a so-called "partial bijection", namely
+     the bijection between the set [count_blocks_to_shift_per_comp, inf) and the set N
+     of all the natural numbers.
+     However, I am defining this bijection 
+     (between [count_blocks_to_shift_per_comp, inf) and N)
+     as a total bijection between
+     {care, dontcare} x N and {care, dontcare} x N.
+     Totalizing it enables us to reuse useful results about total bijections.
    *)
-Variable sigma: addr_t -> addr_t (*{fmap addr_t -> addr_t}*).
-Variable inverse_sigma: addr_t -> addr_t.
 
-Hypothesis cancel_inverse_sigma_sigma: cancel inverse_sigma sigma.
-Hypothesis cancel_sigma_inverse_sigma: cancel sigma inverse_sigma.
-Hypothesis sigma_injective: injective sigma.
+  Variable count_blocks_to_shift_per_comp : nat.
+  
+  Definition care := true.
+  Definition dontcare := false.
 
-(*Definition inverse_sigma (addr: addr_t) : addr_t :=
+  Definition sigma_from_bigger_dom (x: bool * addr_t) : bool * addr_t :=
+    match x with
+    | (c, (cid, bid)) =>
+      if c =? care then
+        if bid <? count_blocks_to_shift_per_comp
+        then (dontcare, (cid, bid))
+        else (care, (cid, bid - count_blocks_to_shift_per_comp))
+      else (dontcare, (cid, bid + count_blocks_to_shift_per_comp))
+    end.
+
+  Definition inv_sigma_from_bigger_dom (x: bool * addr_t) : bool * addr_t :=
+    match x with
+    | (c, (cid, bid)) =>
+      if c =? care then
+        (care, (cid, bid + count_blocks_to_shift_per_comp))
+      else if bid <? count_blocks_to_shift_per_comp
+           then (care, (cid, bid))
+           else (dontcare, (cid, bid - count_blocks_to_shift_per_comp))
+    end.
+
+  Lemma cancel_sigma_from_bigger_dom_inv_sigma_from_bigger_dom :
+    cancel sigma_from_bigger_dom inv_sigma_from_bigger_dom.
+  Proof.
+    unfold cancel. intros [c [cid bid]].
+    destruct c; simpl.
+    - destruct (bid <? count_blocks_to_shift_per_comp) eqn:bid_lt; simpl.
+      + rewrite bid_lt. reflexivity.
+      + rewrite subnK; try reflexivity.
+        assert (le count_blocks_to_shift_per_comp bid) as Hle.
+        { rewrite <- Nat.ltb_ge. assumption. }
+        apply/leP. assumption.
+    - pose proof (leq_addl bid count_blocks_to_shift_per_comp) as H.
+      destruct (bid + count_blocks_to_shift_per_comp <? count_blocks_to_shift_per_comp)
+               eqn:bid_plus_lt; simpl.
+      + pose proof Nat.ltb_lt (addn bid count_blocks_to_shift_per_comp)
+             (count_blocks_to_shift_per_comp) as [Hif _].
+        rewrite bid_plus_lt in Hif. pose proof (Hif Logic.eq_refl) as Hlt. clear Hif.
+        assert (leq (S (addn bid count_blocks_to_shift_per_comp))
+                    count_blocks_to_shift_per_comp) as Hleq.
+        { apply/ltP. assumption. }
+        pose proof (leqP count_blocks_to_shift_per_comp
+                         (addn bid count_blocks_to_shift_per_comp)) as Hcontra.
+        rewrite H in Hcontra. rewrite Hleq in Hcontra.
+        inversion Hcontra.
+      + rewrite addnK. reflexivity.
+  Qed.
+
+  Lemma cancel_inv_sigma_from_bigger_dom_sigma_from_bigger_dom :
+    cancel inv_sigma_from_bigger_dom sigma_from_bigger_dom.
+  Proof.
+    unfold cancel. intros [c [cid bid]]. destruct c; simpl.
+    - pose proof leq_addl bid count_blocks_to_shift_per_comp.
+      assert (bid + count_blocks_to_shift_per_comp <? count_blocks_to_shift_per_comp = false)
+        as Hfalse.
+      { rewrite Nat.ltb_ge. apply/leP. assumption. }
+      rewrite Hfalse. rewrite addnK. reflexivity.
+    - destruct (bid <? count_blocks_to_shift_per_comp) eqn:HNatlt;
+        unfold sigma_from_bigger_dom; simpl.
+      + rewrite HNatlt. reflexivity.
+      + rewrite subnK; try reflexivity.
+        apply/leP. rewrite <- Nat.ltb_ge. assumption.
+  Qed.
+
+  Lemma sigma_from_bigger_dom_bijective : bijective sigma_from_bigger_dom.
+  Proof. apply Bijective with (g := inv_sigma_from_bigger_dom).
+         - exact cancel_sigma_from_bigger_dom_inv_sigma_from_bigger_dom.
+         - exact cancel_inv_sigma_from_bigger_dom_sigma_from_bigger_dom.
+  Qed.
+
+  Lemma inv_sigma_from_bigger_dom_bijective : bijective inv_sigma_from_bigger_dom.
+  Proof. apply Bijective with (g := sigma_from_bigger_dom).
+         - exact cancel_inv_sigma_from_bigger_dom_sigma_from_bigger_dom.
+         - exact cancel_sigma_from_bigger_dom_inv_sigma_from_bigger_dom.
+  Qed.
+
+  
+End ShiftingAsPartialBijection.
+
+
+Definition mem_of_event (e: event) : Memory.t :=
+  match e with
+  | ECall _ _ _ mem _ => mem
+  | ERet _ _ mem _ => mem
+  end.
+
+Definition arg_of_event (e: event) : value :=
+  match e with
+  | ECall _ _ v _ _ => v
+  | ERet _ v _ _ => v
+  end.
+
+Definition addr_of_value (v: value) : {fset addr_t} :=
+  match v with
+  | Ptr (perm, cid, bid, _) =>
+    if perm =? Permission.data then fset1 (cid, bid) else fset0
+  | _ => fset0
+  end.
+
+Inductive addr_shared_so_far : addr_t -> trace event -> Prop :=
+| reachable_from_args_is_shared:
+    forall addr t e,
+      Reachable (mem_of_event e) (addr_of_value (arg_of_event e)) addr ->
+      addr_shared_so_far addr (rcons t e)
+| reachable_from_previously_shared:
+    forall addr addr' t e,
+      addr_shared_so_far addr' t ->
+      Reachable (mem_of_event e) (fset1 addr') addr ->
+      addr_shared_so_far addr (rcons t e).
+
+Section Renaming.
+
+  Variable sigma: addr_t -> addr_t (*{fmap addr_t -> addr_t}*).
+  Variable inverse_sigma: addr_t -> addr_t.
+
+  Hypothesis cancel_inverse_sigma_sigma: cancel inverse_sigma sigma.
+  Hypothesis cancel_sigma_inverse_sigma: cancel sigma inverse_sigma.
+  Hypothesis sigma_injective: injective sigma.
+
+  (*Definition inverse_sigma (addr: addr_t) : addr_t :=
   let dom_sigma := domm sigma in
   if has (fun y => sigma y == Some addr) dom_sigma
   then nth (0,0) dom_sigma (find (fun y => sigma y == Some addr) dom_sigma)
   else addr.
- *)
+   *)
 
-Definition rename_addr (addr: addr_t) : addr_t := sigma addr.
-(*  match sigma addr with
+  Definition rename_addr (addr: addr_t) : addr_t := sigma addr.
+  (*  match sigma addr with
   | Some addr' => addr'
   | None => addr
   end.
-*)
+   *)
 
-Definition inverse_rename_addr (addr: addr_t) := inverse_sigma addr.
+  Definition inverse_rename_addr (addr: addr_t) := inverse_sigma addr.
 
-Definition rename_value_template (rnm_addr : addr_t -> addr_t) (v: value) : value :=
-  match v with
-  | Ptr (perm, cid, bid, off) =>
-    let (cid', bid') := rnm_addr (cid, bid) in
-    Ptr (perm, cid', bid', off)
-  | _ => v
-  end.
+  Definition rename_value_template (rnm_addr : addr_t -> addr_t) (v: value) : value :=
+    match v with
+    | Ptr (perm, cid, bid, off) =>
+      let (cid', bid') := rnm_addr (cid, bid) in
+      Ptr (perm, cid', bid', off)
+    | _ => v
+    end.
 
-Definition rename_value (v: value) : value := rename_value_template rename_addr v.
-              
-Definition inverse_rename_value (v: value) : value :=
-  rename_value_template inverse_rename_addr v.
+  Definition rename_value (v: value) : value := rename_value_template rename_addr v.
+  
+  Definition inverse_rename_value (v: value) : value :=
+    rename_value_template inverse_rename_addr v.
 
-Definition rename_list_values (s: list value) : list value := map rename_value s.
+  Definition rename_list_values (s: list value) : list value := map rename_value s.
 
-Definition inverse_rename_list_values (s: list value) : list value :=
-  map inverse_rename_value s.
+  Definition inverse_rename_list_values (s: list value) : list value :=
+    map inverse_rename_value s.
 
-Lemma inverse_rename_addr_left_inverse addr: inverse_rename_addr (rename_addr addr) = addr.
-Proof.
-  unfold inverse_rename_addr, rename_addr. pose proof (cancel_sigma_inverse_sigma addr). auto.
-Qed.
+  Lemma inverse_rename_addr_left_inverse addr: inverse_rename_addr (rename_addr addr) = addr.
+  Proof.
+    unfold inverse_rename_addr, rename_addr. pose proof (cancel_sigma_inverse_sigma addr). auto.
+  Qed.
 
-(***************************** 
+  (***************************** 
     [DEPRECATED]: sigma was fmap.
 
 Lemma inverse_rename_addr_left_inverse addr:
@@ -105,18 +231,18 @@ Proof.
   - rewrite mem_domm in Haddr. rewrite e_sigma_addr in Haddr. easy.
 Qed.
 
-****************************************)
+   ****************************************)
 
 
-Lemma inverse_rename_addr_right_inverse addr:
-  rename_addr (inverse_rename_addr addr) = addr.
-Proof.
-  unfold inverse_rename_addr, rename_addr. pose proof (cancel_inverse_sigma_sigma addr). auto.
-Qed.
+  Lemma inverse_rename_addr_right_inverse addr:
+    rename_addr (inverse_rename_addr addr) = addr.
+  Proof.
+    unfold inverse_rename_addr, rename_addr. pose proof (cancel_inverse_sigma_sigma addr). auto.
+  Qed.
 
 
 
-(**************************************
+  (**************************************
     [DEPRECATED]: sigma was finmap      
 
 Lemma inverse_rename_addr_right_inverse addr_pre addr:
@@ -139,35 +265,110 @@ Proof.
     apply H in contra. exfalso. assumption.
 Qed.  
 
-*********************************)
+   *********************************)
 
-Definition rename_memory_content_at_addr (m: Memory.t) (addr: Component.id * Block.id)
-  : Memory.t :=
-  match omap rename_list_values (Memory.load_all m addr) with
-  | Some vs => match Memory.store_all m addr vs with
-               | Some m' => m'
-               | None => m
-               end
-  | None => m
-  end.
+  Definition option_rename_value option_v := omap rename_value option_v.
+  Definition option_inverse_rename_value option_v := omap inverse_rename_value option_v.
 
-Fixpoint rename_memory_content_at_addrs (m: Memory.t) (addrs: list (Component.id * Block.id))
-  : Memory.t :=
-  match addrs with
-  | nil => m
-  | cb :: cbs => rename_memory_content_at_addrs (rename_memory_content_at_addr m cb) cbs
-  end.
+  Definition event_renames_event_at_addr addr e e' : Prop :=
+    forall offset,
+      Memory.load (mem_of_event e')
+                  (
+                    Permission.data,
+                    (rename_addr addr).1,
+                    (rename_addr addr).2,
+                    offset
+                  )
+      =
+      option_rename_value
+        (
+          Memory.load (mem_of_event e)
+                      (Permission.data,
+                       addr.1,
+                       addr.2,
+                       offset)
+        ).
 
-Definition rename_memory_addrs (m: Memory.t) (addrs: list (Component.id * Block.id))
-  : Memory.t :=
-  Memory.transfer_memory_blocks m addrs m (map rename_addr addrs).
+  Definition event_inverse_renames_event_at_addr addr' e e' : Prop :=
+    forall offset,
+      option_inverse_rename_value
+        (
+          Memory.load (mem_of_event e')
+                      (Permission.data,
+                       addr'.1,
+                       addr'.2,
+                       offset
+                      )
+        )
+      =
+      Memory.load (mem_of_event e)
+                  (Permission.data,
+                   (inverse_rename_addr addr').1,
+                   (inverse_rename_addr addr').2,
+                   offset
+                  ).
 
-Definition rename_memory_subgraph (m: Memory.t) (addrs: list (Component.id * Block.id))
-  : Memory.t :=
-  rename_memory_content_at_addrs (rename_memory_addrs m addrs) (map rename_addr addrs).
+  Inductive traces_rename_each_other :
+    trace event -> trace event -> Prop :=
+  | nil_renames_nil: traces_rename_each_other nil nil
+  | rcons_renames_rcons:
+      forall tprefix e tprefix' e',
+        traces_rename_each_other tprefix tprefix' ->
+        (
+          forall addr, addr_shared_so_far addr (rcons tprefix e) ->
+                       (
+                         event_renames_event_at_addr addr e e'
+                         /\
+                         addr_shared_so_far (rename_addr addr) (rcons tprefix' e')
+                       )
+        )
+        ->
+        (
+          forall addr', addr_shared_so_far addr' (rcons tprefix' e') ->
+                        (
+                          event_inverse_renames_event_at_addr addr' e e'
+                          /\
+                          addr_shared_so_far (inverse_rename_addr addr')
+                                             (rcons tprefix e)
+                        )
+        )
+        ->
+        traces_rename_each_other (rcons tprefix e) (rcons tprefix' e').
+  
 
-(* [DynShare]: TODO:
-   Is this lemma needed?
+
+
+
+  (******************************************
+     [DEPRECATED]: Memory renaming has now been defined as part of event renaming.
+
+  Definition rename_memory_content_at_addr (m: Memory.t) (addr: Component.id * Block.id)
+    : Memory.t :=
+    match omap rename_list_values (Memory.load_all m addr) with
+    | Some vs => match Memory.store_all m addr vs with
+                 | Some m' => m'
+                 | None => m
+                 end
+    | None => m
+    end.
+
+  Fixpoint rename_memory_content_at_addrs (m: Memory.t) (addrs: list (Component.id * Block.id))
+    : Memory.t :=
+    match addrs with
+    | nil => m
+    | cb :: cbs => rename_memory_content_at_addrs (rename_memory_content_at_addr m cb) cbs
+    end.
+
+  Definition rename_memory_addrs (m: Memory.t) (addrs: list (Component.id * Block.id))
+    : Memory.t :=
+    Memory.transfer_memory_blocks m addrs m (map rename_addr addrs).
+
+  Definition rename_memory_subgraph (m: Memory.t) (addrs: list (Component.id * Block.id))
+    : Memory.t :=
+    rename_memory_content_at_addrs (rename_memory_addrs m addrs) (map rename_addr addrs).
+
+  (* [DynShare]: TODO:
+   Is the following lemma needed?
    This lemma may be a bit too tedious to prove.
 
    Alternatively, I will experiment with representing the trace renaming
@@ -176,52 +377,23 @@ Definition rename_memory_subgraph (m: Memory.t) (addrs: list (Component.id * Blo
    * Mem_Renames_Mem
    * Addr_shared_so_far, which itself will use the definition of
    * Reachable
-*)
+   *)
+  Lemma reachable_nodes_nat_rename m start:
+    fset (
+        reachable_nodes_nat
+          (rename_memory_subgraph m (reachable_nodes_nat m start))
+          (rename_addr start)
+      )
+    =
+    fset (map rename_addr (reachable_nodes_nat m start)).
+  Admitted.
 
-Lemma reachable_nodes_nat_rename m start:
-  fset (
-      reachable_nodes_nat
-        (rename_memory_subgraph m (reachable_nodes_nat m start))
-        (rename_addr start)
-    )
-  =
-  fset (map rename_addr (reachable_nodes_nat m start)).
-Admitted.
+   *********************************************)
 
 End Renaming.
 
-Definition mem_of_event (e: event) : Memory.t :=
-  match e with
-  | ECall _ _ _ mem _ => mem
-  | ERet _ _ mem _ => mem
-  end.
-
-Definition arg_of_event (e: event) : value :=
-  match e with
-  | ECall _ _ v _ _ => v
-  | ERet _ v _ _ => v
-  end.
-
-Definition addr_of_value (v: value) : {fset addr_t} :=
-  match v with
-  | Ptr (perm, cid, bid, _) =>
-    if perm =? Permission.data then fset1 (cid, bid) else fset0
-  | _ => fset0
-  end.
-
-Inductive addr_shared_so_far : addr_t -> trace event -> Prop :=
-| reachable_from_args_is_shared:
-    forall addr t e,
-      Reachable (mem_of_event e) (addr_of_value (arg_of_event e)) addr ->
-      addr_shared_so_far addr (rcons t e)
-| reachable_from_previously_shared:
-    forall addr addr' t e,
-      addr_shared_so_far addr' t ->
-      Reachable (mem_of_event e) (fset1 addr') addr ->
-      addr_shared_so_far addr (rcons t e).
-
 (* [DynShare] 
-   This definition is NOT needed when we define a trace relation that
+   The following definition is NOT needed when we define a trace relation that
    (implicitly) specifies the shared part of the memory.
    
    It would be needed though if instead we define a trace semantics
@@ -240,82 +412,4 @@ Definition shared_part_of_memory
                       /\
                       (~ addr_shared_so_far addr t) ->
                       Memory.load mshr (Permission.data, addr.1, addr.2, offset) = None.
-                                  
-Definition option_rename_value sigma option_v :=
-  match option_v with
-  | Some v => Some (rename_value sigma v)
-  | None => None
-  end.
-
-Definition option_inverse_rename_value sigma option_v :=
-  match option_v with
-  | Some v => Some (inverse_rename_value sigma v)
-  | None => None
-  end.
-
-Definition event_renames_event_at_addr sigma addr e e' : Prop :=
-  forall offset,
-  Memory.load (mem_of_event e')
-              (
-                Permission.data,
-                (rename_addr sigma addr).1,
-                (rename_addr sigma addr).2,
-                offset
-              )
-  =
-  option_rename_value sigma
-                      (
-                        Memory.load (mem_of_event e)
-                                    (Permission.data,
-                                     addr.1,
-                                     addr.2,
-                                     offset)
-                      ).
-
-Definition event_inverse_renames_event_at_addr sigma addr' e e' : Prop :=
-  forall offset,
-    option_inverse_rename_value sigma
-                                (
-                                  Memory.load (mem_of_event e')
-                                              (Permission.data,
-                                               addr'.1,
-                                               addr'.2,
-                                               offset
-                                              )
-                                )
-    =
-    Memory.load (mem_of_event e)
-                (Permission.data,
-                 (inverse_rename_addr sigma addr').1,
-                 (inverse_rename_addr sigma addr').2,
-                 offset
-                ).
-                      
-Inductive traces_rename_each_other
-          (sigma: addr_t -> addr_t (*{fmap addr_t -> addr_t}*)) :
-  trace event -> trace event -> Prop :=
-| nil_renames_nil: traces_rename_each_other sigma nil nil
-| rcons_renames_rcons:
-    forall tprefix e tprefix' e',
-      traces_rename_each_other sigma tprefix tprefix' ->
-      (
-        forall addr, addr_shared_so_far addr (rcons tprefix e) ->
-                     (
-                       event_renames_event_at_addr sigma addr e e'
-                       /\
-                       addr_shared_so_far (rename_addr sigma addr) (rcons tprefix' e')
-                     )
-      )
-      ->
-      (
-        forall addr', addr_shared_so_far addr' (rcons tprefix' e') ->
-                      (
-                        event_inverse_renames_event_at_addr sigma addr' e e'
-                        /\
-                        addr_shared_so_far (inverse_rename_addr sigma addr')
-                                           (rcons tprefix e)
-                      )
-      )
-      ->
-      traces_rename_each_other sigma (rcons tprefix e) (rcons tprefix' e').
-
+                                
